Finish verification of naive pattern compiler
Including proof that it preserves set-global operations,
the key reason for the naive version

compiler/backend/proofs/flat_patternProofScript.sml
@@ -1353,8 +1353,6 @@ Proof
   \\ qexists_tac `0` \\ simp []
 QED
 
-(* correctness of naive pattern encoding *)
-
 Theorem naive_pattern_match_correct:
   !t mats vs exp res bindings.
   naive_pattern_match t mats = exp /\
@@ -1442,6 +1440,25 @@ Proof
   \\ rpt (CASE_TAC \\ fs [])
 QED
 
+Theorem pmatch_rows_same_FST:
+  !pats pats2. MAP FST pats = MAP FST pats2 ==>
+  case pmatch_rows pats s v of
+    | Match_type_error => pmatch_rows pats2 s v = Match_type_error
+    | No_match => pmatch_rows pats2 s v = No_match
+    | Match (env,p,e) => ?i. i < LENGTH pats2 /\ EL i pats = (p, e) /\
+        pmatch_rows pats2 s v = Match (env, EL i pats2)
+Proof
+  Induct \\ simp [pmatch_rows_def]
+  \\ gen_tac \\ Cases \\ simp []
+  \\ Cases_on `h` \\ Cases_on `h'`
+  \\ simp [pmatch_rows_def]
+  \\ rw []
+  \\ first_x_assum drule
+  \\ rpt (CASE_TAC \\ fs [])
+  \\ rw []
+  \\ TRY (qexists_tac `0` \\ simp [] \\ NO_TAC)
+  \\ TRY (qexists_tac `SUC i` \\ simp [] \\ NO_TAC)
+QED
 
 Theorem evaluate_compile_pats:
   pmatch_rows pats s v <> Match_type_error /\
@@ -1456,9 +1473,7 @@ Theorem evaluate_compile_pats:
   evaluate env s [case pmatch_rows pats s v of
     | Match (env', p', e') => compile_pat_rhs t N exp (p', e')
     | _ => default_x]
-
 Proof
-
   rw [compile_pats_def]
   \\ fs [prev_cfg_rel_def]
   >- (
@@ -1466,12 +1481,14 @@ Proof
     drule (SIMP_RULE bool_ss [] naive_pattern_matches_correct)
     \\ disch_then (fn t => DEP_REWRITE_TAC [t])
     \\ simp []
-
-    (* need a different rule about pmatch rows *)
-
+    \\ qmatch_goalsub_abbrev_tac `ZIP map_pats`
+    \\ Q.ISPECL_THEN [`s`, `v`, `ZIP map_pats`, `pats`] mp_tac
+        (Q.GENL [`s`, `v`] pmatch_rows_same_FST)
+    \\ fs [markerTheory.Abbrev_def, MAP_ZIP]
+    \\ rpt (CASE_TAC \\ fs [])
+    \\ rw []
+    \\ rfs [EL_ZIP, EL_MAP]
   )
-
-
   \\ drule (Q.SPECL [`pats`, `0`] pmatch_rows_encode)
   \\ rpt (disch_then drule)
   \\ TOP_CASE_TAC
@@ -1483,7 +1500,6 @@ Proof
   \\ EVERY_CASE_TAC \\ fs []
   \\ rw [] \\ fs []
   \\ simp [EL_MAP]
-
 QED
 
 Theorem pmatch_rows_IMP_pmatch:
@@ -1496,8 +1512,8 @@ Proof
 QED
 
 Theorem compile_match_pmatch_rows:
-  !pats k pats2 res.
-  compile_match prev_cfg pats = (k, pats2) /\
+  !pats k sg pats2 res.
+  compile_match prev_cfg pats = (k, sg, pats2) /\
   v_rel cfg v v' /\
   state_rel cfg s t /\
   k <= N /\
@@ -1529,12 +1545,12 @@ Proof
 QED
 
 Theorem compile_match_EL:
-  !pats pats2 k i.
-  compile_match cfg pats = (k, pats2) /\
+  !pats pats2 k sg i.
+  compile_match cfg pats = (k, sg, pats2) /\
   i < LENGTH pats /\
   EL i pats = (pat, exp) ==>
-  ?exp_i exp'.
-  compile_exps cfg [exp] = (exp_i, [exp']) /\
+  ?exp_i sg exp'.
+  compile_exps cfg [exp] = (exp_i, sg, [exp']) /\
   EL i pats2 = (pat, exp') /\
   exp_i <= k /\ max_dec_name (pat_bindings pat []) <= k
 Proof
@@ -1655,9 +1671,9 @@ Proof
 QED
 
 Theorem compile_exps_evaluate:
-  !env1 ^s1 xs t1 r1 i ys N env2 ^s2 prev_cfg.
+  !env1 ^s1 xs t1 r1 i sg ys N env2 ^s2 prev_cfg.
     evaluate env1 s1 xs = (t1, r1) /\
-    compile_exps prev_cfg xs = (i, ys) /\
+    compile_exps prev_cfg xs = (i, sg, ys) /\
     r1 <> Rerr (Rabort Rtype_error) /\
     env_rel cfg N env1 env2 /\ state_rel cfg s1 s2 /\ i < N /\
     prev_cfg_rel prev_cfg cfg /\
@@ -1676,7 +1692,6 @@ Theorem compile_exps_evaluate:
       EVERY (v_cons_in_c s2.c) (result_vs r2) /\
       t2.c = s2.c
 Proof
-
   ho_match_mp_tac evaluate_ind
   \\ simp [evaluate_def, compile_exps_def, result_vs_def]
   \\ rpt (gen_tac ORELSE disch_tac ORELSE conj_tac)
@@ -1971,9 +1986,9 @@ Proof
   \\ rveq \\ fs [OPTREL_def]
   >- (
     (* Dlet *)
-    Cases_on `compile_exps cfg [e]`
+    `?N sg exps. compile_exps cfg [e] = (N, sg, exps)` by metis_tac [pair_CASES]
     \\ drule_then drule compile_exps_evaluate
-    \\ disch_then (qspecl_then [`cfg`, `q + 1`, `<| v := [] |>`, `s2`] mp_tac)
+    \\ disch_then (qspecl_then [`cfg`, `N + 1`, `<| v := [] |>`, `s2`] mp_tac)
     \\ simp [env_rel_def, ALOOKUP_rel_empty, prev_cfg_rel_refl]
     \\ impl_tac >- (CCONTR_TAC \\ fs [])
     \\ rw [prev_cfg_rel_refl]
@@ -2181,18 +2196,12 @@ QED
 
 (* set_globals and esgc properties *)
 
-Theorem elist_globals_REVERSE:
-  elist_globals (REVERSE es) = elist_globals es
-Proof
-  Induct_on `es` \\ simp [elist_globals_append, COMM_BAG_UNION]
-QED
-
-
-Definition dtree_rhss_def:
-  dtree_rhss (Leaf n) = [SUC n] /\
-  dtree_rhss (If _ dt1 dt2) = dtree_rhss dt1 ++ dtree_rhss dt2 /\
-  dtree_rhss Fail = [0] /\
-  dtree_rhss TypeFail = []
+Definition dtree_indexes_ok_def:
+  dtree_indexes_ok n (Leaf i) = (i < n) /\
+  dtree_indexes_ok n (If _ dt1 dt2) =
+  (dtree_indexes_ok n dt1 /\ dtree_indexes_ok n dt2) /\
+  dtree_indexes_ok n Fail = T /\
+  dtree_indexes_ok n TypeFail = T
 End
 
 Theorem set_globals_decode_pos:
@@ -2218,72 +2227,15 @@ Proof
   \\ simp [set_globals_decode_test, set_globals_decode_pos]
 QED
 
-Theorem set_globals_decode_dtree:
-  set_globals (decode_dtree t exps (Var_local t' nm) dflt dtree)
-  =
-  elist_globals (MAP (\i. EL i (dflt :: exps)) (dtree_rhss dtree))
+Theorem set_globals_decode_dtree_empty:
+  set_globals x = {||} /\ set_globals dflt = {||} /\
+  elist_globals exps = {||} /\ dtree_indexes_ok (LENGTH exps) dtree ==>
+  set_globals (decode_dtree t exps x dflt dtree) = {||}
 Proof
   Induct_on `dtree`
-  \\ simp [decode_dtree_def, dtree_rhss_def]
-  \\ simp [elist_globals_append, set_globals_decode_guard]
-QED
-
-Theorem elist_globals_unshuffle_LIST_TO_BAG:
-  !xs ys. LIST_TO_BAG xs = LIST_TO_BAG ys ==>
-  elist_globals xs = elist_globals ys
-Proof
-  Induct \\ rw []
-  >- (
-    Cases_on `ys` \\ fs []
-  )
-  \\ first_assum (mp_tac o Q.AP_TERM `\bg. BAG_IN h bg`)
-  \\ rw [IN_LIST_TO_BAG]
-  \\ fs [MEM_SPLIT]
-  \\ first_x_assum (qspec_then `l1 ++ l2` mp_tac)
-  \\ fs [LIST_TO_BAG_APPEND, BAG_UNION_INSERT]
-  \\ simp_tac (bool_ss ++ bagSimps.BAG_ss) [elist_globals_append]
-  \\ simp []
-QED
-
-Theorem BAG_IMAGE_unshuffle_MAP_EL:
-  !N. N <= LENGTH xs ==>
-  BAG_IMAGE (\i. EL i xs) (LIST_TO_BAG (COUNT_LIST N)) =
-  LIST_TO_BAG (TAKE N xs)
-Proof
-  Induct
-  \\ rw [COUNT_LIST_SNOC]
-  \\ fs [SNOC_APPEND, LIST_TO_BAG_APPEND, GSYM SNOC_EL_TAKE]
-QED
-
-Theorem elist_globals_unshuffle_MAP_EL:
-  LIST_TO_BAG ns = LIST_TO_BAG (COUNT_LIST (LENGTH exps)) ==>
-  elist_globals (MAP (\i. EL i exps) ns) =
-  elist_globals exps
-Proof
-  rw []
-  \\ irule elist_globals_unshuffle_LIST_TO_BAG
-  \\ simp [LIST_TO_BAG_MAP, BAG_IMAGE_unshuffle_MAP_EL]
-QED
-
-Theorem dtree_rhss_bag:
-  LIST_TO_BAG (dtree_rhss (top_level_pat_compile h ps)) =
-  LIST_TO_BAG (COUNT_LIST (SUC (LENGTH ps)))
-Proof
-  cheat
-QED
-
-Theorem SET_OF_LIST_TO_BAG:
-  SET_OF_BAG (LIST_TO_BAG xs) = set xs
-Proof
-  Induct_on `xs` \\ simp [SET_OF_BAG_INSERT]
-QED
-
-Theorem dtree_rhss_set:
-  set (dtree_rhss (top_level_pat_compile h ps)) ⊆
-  count (SUC (LENGTH ps))
-Proof
-  simp [GSYM SET_OF_LIST_TO_BAG, dtree_rhss_bag]
-  \\ simp [SET_OF_LIST_TO_BAG, COUNT_LIST_COUNT]
+  \\ simp [decode_dtree_def, dtree_indexes_ok_def]
+  \\ simp [set_globals_decode_guard]
+  \\ simp [elist_globals_eq_empty, EL_MEM]
 QED
 
 Theorem inv_on_FOLDR:
@@ -2308,27 +2260,64 @@ Proof
   \\ fs [EVERY_MAP, ELIM_UNCURRY]
 QED
 
-Theorem set_globals_compile_pats:
-  set_globals (compile_pats cfg t N (Var_local t' nm) dflt ps) =
+Theorem set_globals_naive_pattern_match:
+  !t xs. EVERY (\v. set_globals (SND v) = {||}) xs ==>
+  set_globals (naive_pattern_match t xs) = {||}
+Proof
+  ho_match_mp_tac naive_pattern_match_ind
+  \\ simp [naive_pattern_match_def, op_gbag_def, Bool_def]
+  \\ rw []
+  \\ fs []
+  \\ fs [EVERY_EL, op_gbag_def]
+QED
+
+Theorem set_globals_naive_pattern_matches:
+  set_globals x = {||} ==>
+  set_globals (naive_pattern_matches t x ps dflt) =
   elist_globals (dflt :: MAP SND ps)
 Proof
-  simp [compile_pats_def, set_globals_decode_dtree]
-  \\ simp [elist_globals_unshuffle_MAP_EL, dtree_rhss_bag]
-  \\ simp [compile_pat_rhs_def]
-  \\ simp [elist_globals_FOLDR]
-  \\ irule FOLDR_CONG
-  \\ simp []
-  \\ simp [MAP_MAP_o]
-  \\ irule MAP_CONG
-  \\ simp [FORALL_PROD, compile_pat_rhs_def, set_globals_compile_pat_bindings]
+  Induct_on `ps`
+  \\ simp [FORALL_PROD, naive_pattern_matches_def,
+        set_globals_naive_pattern_match]
+  \\ simp_tac (bool_ss ++ bagSimps.BAG_ss) []
+QED
+
+Theorem dtree_indexes_ok:
+  LENGTH pats <= N ==>
+  dtree_indexes_ok N (top_level_pat_compile cfg.pat_heuristic pats)
+Proof
+  cheat
+QED
+
+Theorem set_globals_compile_pats:
+  (~ naive ==> elist_globals (dflt :: MAP SND ps) = {||}) /\
+  set_globals x = {||} ==>
+  set_globals (compile_pats cfg naive t N x dflt ps) =
+  elist_globals (dflt :: MAP SND ps)
+Proof
+  simp [compile_pats_def]
+  \\ rw []
+  >- (
+    simp [set_globals_naive_pattern_matches, MAP_ZIP]
+    \\ simp [elist_globals_FOLDR]
+    \\ irule FOLDR_CONG
+    \\ simp [MAP_MAP_o]
+    \\ irule MAP_CONG
+    \\ simp [FORALL_PROD, compile_pat_rhs_def, set_globals_compile_pat_bindings]
+  )
+  \\ DEP_REWRITE_TAC [set_globals_decode_dtree_empty]
+  \\ simp [dtree_indexes_ok]
+  \\ fs [elist_globals_eq_empty, MEM_MAP, PULL_EXISTS]
+  \\ fs [FORALL_PROD, compile_pat_rhs_def, set_globals_compile_pat_bindings]
+  \\ metis_tac []
 QED
 
 Theorem compile_exps_elist_globals:
-  (!cfg exps N exps'. compile_exps cfg exps = (N, exps')
+  (!cfg exps N sg exps'. compile_exps cfg exps = (N, sg, exps')
   ==>
   elist_globals exps' = elist_globals exps)
   /\
-  (!cfg m N m'. compile_match cfg m = (N, m')
+  (!cfg m N sg m'. compile_match cfg m = (N, sg, m')
   ==>
   elist_globals (MAP SND m') = elist_globals (MAP SND m))
 Proof
@@ -2337,17 +2326,18 @@ Proof
   \\ rw []
   \\ rpt (pairarg_tac \\ fs [])
   \\ rveq \\ fs []
-  \\ fs [set_globals_compile_pats]
   \\ imp_res_tac flat_patternTheory.LENGTH_compile_exps_IMP
   \\ fs [quantHeuristicsTheory.LIST_LENGTH_2, elist_globals_REVERSE]
   \\ rveq \\ fs []
+  \\ TRY (DEP_REWRITE_TAC [set_globals_compile_pats]
+    \\ imp_res_tac compile_exps_set_globals
+    \\ simp [])
   \\ simp [elist_globals_FOLDR] \\ irule FOLDR_CONG
   \\ simp [MAP_MAP_o] \\ irule MAP_CONG
   \\ simp [FORALL_PROD] \\ rw []
-  \\ qmatch_goalsub_abbrev_tac `compile_exps cfg [inner_exp]`
-  \\ Cases_on `compile_exps cfg [inner_exp]`
+  \\ rpt (pairarg_tac \\ fs [])
   \\ first_x_assum drule
-  \\ imp_res_tac flat_patternTheory.LENGTH_compile_exps_IMP
+  \\ imp_res_tac LENGTH_compile_exps_IMP
   \\ fs [quantHeuristicsTheory.LIST_LENGTH_2, elist_globals_REVERSE]
 QED
 
@@ -2365,7 +2355,7 @@ Proof
   \\ last_x_assum drule \\ rw []
   \\ rveq \\ fs []
   \\ qmatch_goalsub_abbrev_tac `compile_exps cfg [exp]`
-  \\ Cases_on `compile_exps cfg [exp]`
+  \\ `?N sg e'. compile_exps cfg [exp] = (N, sg, e')` by metis_tac [pair_CASES]
   \\ imp_res_tac LENGTH_compile_exps_IMP
   \\ drule (CONJUNCT1 compile_exps_elist_globals)
   \\ fs [quantHeuristicsTheory.LIST_LENGTH_2]
@@ -2394,12 +2384,12 @@ QED
 
 Theorem esgc_free_decode_dtree:
   esgc_free v_exp /\ esgc_free dflt /\ EVERY esgc_free exps /\
-  set (dtree_rhss dtree) SUBSET count (SUC (LENGTH exps)) ==>
+  dtree_indexes_ok (LENGTH exps) dtree ==>
   esgc_free (decode_dtree t exps v_exp dflt dtree)
 Proof
   Induct_on `dtree`
-  \\ simp [decode_dtree_def]
-  \\ simp [esgc_free_decode_guard, dtree_rhss_def, EVERY_EL]
+  \\ simp [decode_dtree_def, dtree_indexes_ok_def]
+  \\ simp [esgc_free_decode_guard, EVERY_EL]
 QED
 
 Theorem esgc_free_compile_pat_bindings:
@@ -2417,23 +2407,35 @@ Proof
   \\ fs [EVERY_MAP, ELIM_UNCURRY]
 QED
 
+Theorem esgc_free_naive_pattern_match:
+  !t xs. EVERY esgc_free (MAP SND xs) ==>
+  esgc_free (naive_pattern_match t xs)
+Proof
+  ho_match_mp_tac naive_pattern_match_ind
+  \\ simp [naive_pattern_match_def, Bool_def]
+  \\ rw []
+  \\ fs [EVERY_EL]
+QED
+
+Theorem esgc_free_naive_pattern_matches:
+  !t x xs dflt. EVERY esgc_free (x :: dflt :: MAP SND xs) ==>
+  esgc_free (naive_pattern_matches t x xs dflt)
+Proof
+  ho_match_mp_tac naive_pattern_matches_ind
+  \\ simp [naive_pattern_matches_def, esgc_free_naive_pattern_match]
+QED
+
 Theorem esgc_free_compile_pats:
   esgc_free dflt /\ EVERY esgc_free (MAP SND ps) ==>
-  esgc_free (compile_pats cfg t N (Var_local t' nm) dflt ps)
+  esgc_free (compile_pats cfg naive t N (Var_local t' nm) dflt ps)
 Proof
   rw [compile_pats_def]
-  \\ DEP_REWRITE_TAC [esgc_free_decode_dtree]
-  \\ rw []
-  >- (
-    fs [EVERY_MAP]
-    \\ fs [EVERY_MEM, FORALL_PROD]
-    \\ rw [EVERY_MEM, FORALL_PROD, compile_pat_rhs_def]
-    \\ irule esgc_free_compile_pat_bindings
-    \\ res_tac
-    \\ simp []
-  )
-  \\ irule (MATCH_MP (hd (RES_CANON SUBSET_TRANS)) dtree_rhss_set)
-  \\ simp []
+  \\ DEP_REWRITE_TAC [esgc_free_decode_dtree, esgc_free_naive_pattern_matches]
+  \\ simp [MAP_ZIP, dtree_indexes_ok]
+  \\ fs [EVERY_MAP]
+  \\ first_x_assum (fn t => mp_tac t \\ match_mp_tac MONO_EVERY)
+  \\ simp [FORALL_PROD, compile_pat_rhs_def]
+  \\ simp [esgc_free_compile_pat_bindings]
 QED
 
 Theorem compile_exps_esgc_free:
